test.lean
@@ -1,2 +1,0 @@
-import Mathlib.Computability.TMComputable
-#check Turing.FinTM2
